

1.

(a) $\Delta x = 1/4 = 0.25$, $x_0 = 0$, $x_1 = 0.25$, $x_2 = 0.5$, $x_3 = 0.75$, $x_4 = 1$.

$$\begin{aligned} S_4 &= \frac{\Delta x}{3}(f(x_0) + 4f(x_1) + 2f(x_2) + 4f(x_3) + f(x_4)) \\ &= \frac{0.25}{4}(0 + 4(0.25)^2 + 2(0.5)^2 + 4(0.75)^2 + 1) \\ &= \frac{1}{3}. \end{aligned}$$

(b) $f(x) = \sin(x^2)$, $f'(x) = 2x \cos(x^2)$, $f''(x) = 2 \cos(x^2) - 4x^2 \sin(x^2)$. So,

$$|f''(x)| = |2 \cos(x^2) - 4x^2 \sin(x^2)| \leq |2 \cos(x^2)| + |-4x^2 \sin(x^2)| \leq 2 + 4 = 6.$$

Using $K = 6$ in the Error Bound, we want to find an n such that

$$\begin{aligned} |E_M| &\leq \frac{K(b-a)^3}{24n^2} < 10^{-3} \\ \iff \frac{6}{24n^2} < 10^{-3} &\iff n > 15.811. \end{aligned}$$

We can choose $n = 16$.

2.

(a) Note that $x^2 + 6x = (x + 3)^2 - 3^2$. Use Trigo substitution. Set $x + 3 = 3 \sec \theta$.

$$\begin{aligned} \int \frac{1}{\sqrt{x^2 + 6x}} dx &= \int \frac{1}{\sqrt{3^2 \sec^2 \theta - 3^2}} \cdot 3 \sec \theta \tan \theta d\theta \\ &= \int \sec \theta d\theta \\ &= \ln |\sec \theta + \tan \theta| + C \\ &= \ln \left| \frac{x+3}{3} + \frac{\sqrt{x^2+6x}}{3} \right| + C \\ &= \ln |x+3+\sqrt{x^2+6x}| + C' \end{aligned}$$

(b) Note that the partial fraction decomposition of $\frac{1}{x^2(x^2+25)}$ has the form $\frac{A}{x} + \frac{B}{x^2} + \frac{Cx+D}{x^2+25}$. Solving for A , B , C , D , we have

$$\frac{1}{x^2(x^2+25)} = \frac{1}{25x^2} - \frac{1}{25(x^2+25)}.$$

Integrating, we have

$$\begin{aligned} \int \frac{1}{x^2(x^2+25)} dx &= \int \frac{1}{25x^2} dx - \frac{1}{25} \int \frac{1}{x^2+25} dx \\ &= -\frac{1}{25x} - \frac{1}{125} \tan^{-1} \left(\frac{x}{5} \right) + C. \end{aligned}$$

3.

(a) Note that $a_n = \frac{2n^2+3n}{\sqrt{n^7+1}} \leq \frac{2n^2+3n^2}{\sqrt{n^7}} = \frac{5}{n^{1.5}}$. Since $\sum \frac{5}{n^{1.5}}$ converges (it is a p -series with $p = 1.5 > 1$), by Comparison test, the given series $\sum a_n$ is convergent.

(b) Let $a_n = \tan\left(\frac{n\pi}{4n+\sqrt{n}}\right)$. Since $\tan x$ is continuous at $\pi/4$, we have

$$\lim_{n \rightarrow \infty} a_n = \tan\left(\lim_{n \rightarrow \infty} \frac{n\pi}{4n+\sqrt{n}}\right) = \tan\left(\lim_{n \rightarrow \infty} \frac{\pi}{4+1/\sqrt{n}}\right) = \tan(\pi/4) = 1.$$

Since the term a_n does not vanish, the series $\sum a_n$ is divergent.

(c) Let $a_n = \frac{1}{4^n-3^n}$. Let $b_n = 1/4^n$. Then

$$\lim_{n \rightarrow \infty} \frac{a_n}{b_n} = \lim_{n \rightarrow \infty} \frac{4^n}{4^n-3^n} = \lim_{n \rightarrow \infty} \frac{1}{1-\left(\frac{3}{4}\right)^n} = 1 > 0.$$

By the Limit Comparison Test, the series $\sum a_n$ converges since the series $\sum \frac{1}{4^n}$ converges (it is a geometric series).

4.

(i) Prove by induction on $n \geq 1$ that $0 < a_n < 6$. When $n = 1$, this is clear since $0 < a_1 = 4 < 6$. Assume that $0 < a_n < 6$. Then

$$0 < \sqrt{30} < a_{n+1} = \sqrt{a_n + 30} < \sqrt{6 + 30} = 6.$$

(ii) For any $n \geq 1$, we have

$$a_{n+1} = \sqrt{a_n + 30} = \sqrt{a_n + 6 + 6 + 6 + 6 + 6} > \sqrt{a_n + a_n + a_n + a_n + a_n + a_n} = \sqrt{6a_n} > \sqrt{a_n a_n} = a_n.$$

Thus, $\{a_n\}$ is increasing.

(iii) Let $L = \lim_{n \rightarrow \infty} a_n$. Note that $L \geq 0$. Since \sqrt{x} is continuous at $L + 30$, we deduce that

$$\begin{aligned} \lim_{n \rightarrow \infty} a_{n+1} &= \lim_{n \rightarrow \infty} \sqrt{a_n + 30} = \sqrt{\lim_{n \rightarrow \infty} a_n + 30} \\ L &= \sqrt{L + 30} \implies L = \frac{1 + \sqrt{121}}{2} = 6. \end{aligned}$$

5.

(a) Let $a_n = \frac{n^6(x-5)^n}{n^8+1}$. Then

$$\begin{aligned} \left| \frac{a_{n+1}}{a_n} \right| &= \frac{(n+1)^6|x-5|^{n+1}}{(n+1)^8+1} \cdot \frac{n^8+1}{n^6|x-5|^n} \\ &= \frac{(n+1)^6}{n^6} \cdot \frac{n^8+1}{(n+1)^8+1} \cdot |x-5| \\ &= \left(1 + \frac{1}{n}\right)^6 \cdot \frac{1 + \frac{1}{n^8}}{\left(1 + \frac{1}{n}\right)^8 + \frac{1}{n^8}} \cdot |x-5| \\ &\rightarrow |x-5|. \end{aligned}$$

By the Ratio Test, the series converges (absolutely) if $|x-5| < 1$, i.e. if $4 < x < 6$; diverges if $x < 4$ or $x > 6$.

We now check the convergence at the point $x = 4$, $x = 6$.

If $x = 4$, the series becomes $\sum_{n=0}^{\infty} (-1)^n b_n$, where $b_n = \frac{n^6}{n^8+1}$. Let $f(x) = \frac{x^6}{x^8+1}$. Then

$$f'(x) = \frac{6x^5(x^8+1) - x^6(8x^7)}{(x^8+1)^2} = \frac{x^5(6-2x^3)}{(x^8+1)^2}$$

Note that for $x > 3^{1/3}$, $f'(x) < 0$. In particular, $f(x)$ is decreasing on $[2, \infty)$. So the sequence $\{b_n\}$ is ultimately decreasing, and by the Alternating Series Test, the series $\sum (-1)^n b_n$ converges.

If $x = 6$, the series becomes $\sum_{n=0}^{\infty} b_n$, where $b_n = \frac{n^6}{n^8+1}$. Since $b_n = \frac{n^6}{n^8+1} < \frac{n^6}{n^8} = \frac{1}{n^2}$ and the series $\sum \frac{1}{n^2}$ is convergent (p -series), the series $\sum b_n$ converges by Comparison Test. This implies that the series $\sum (-1)^n b_n$ converges absolutely.

The interval of convergence is $[4, 6]$. The series also converges absolutely on the the interval $[4, 6]$.

(b) Since $\sum |a_n|$ converges, we have $|a_n| \rightarrow 0$, and so $a_n \rightarrow 0$. Thus, eventually $a_n^2 \leq |a_n|$ for $n > N$ for some number N . By Comparison Test, the series $\sum a_n^2$ converges.

Q6.

(a)

$$\begin{aligned}
 f(x) &= \frac{1}{4+3x} = \frac{1}{10+3(x-2)} = \frac{1}{10} \cdot \frac{1}{1 - \left(-\frac{3}{10}(x-2)\right)} \\
 &= \frac{1}{10} \sum_{n=0}^{\infty} \left(-\frac{3}{10}(x-2)\right)^n = \sum_{n=0}^{\infty} \frac{(-1)^n 3^n}{10^{n+1}} (x-2)^n
 \end{aligned}$$

(b)

$$\begin{aligned}
 \frac{1}{1+\sin x} &= \frac{1}{1-(-\sin x)} = 1 - \sin x + (\sin x)^2 - (\sin x)^3 + (\sin x)^4 - \dots \\
 &= 1 - \left(x - \frac{x^3}{3!} + \frac{x^5}{5!} - \frac{x^7}{7!} + \dots\right) \\
 &\quad + \left(x - \frac{x^3}{3!} + \frac{x^5}{5!} - \frac{x^7}{7!} + \dots\right)^2 \\
 &\quad - \left(x - \frac{x^3}{3!} + \frac{x^5}{5!} - \frac{x^7}{7!} + \dots\right)^3 \\
 &\quad + \left(x - \frac{x^3}{3!} + \frac{x^5}{5!} - \frac{x^7}{7!} + \dots\right)^4 + \dots \\
 &= 1 - x + x^2 + \left(\frac{1}{3!} - 1\right)x^3 + \left(-\frac{2}{3!} + 1\right)x^4 \\
 &= 1 - x + x^2 - \frac{5}{6}x^3 + \frac{2}{3}x^4 + \dots
 \end{aligned}$$

(c)

$$\begin{aligned}
 \sum_{n=0}^{\infty} n e^{-nx} &= -\frac{d}{dx} \sum_{n=0}^{\infty} (e^{-nx}) \\
 &= -\frac{d}{dx} \sum_{n=0}^{\infty} (e^{-x})^n \\
 &= -\frac{d}{dx} \left(\frac{1}{1 - e^{-x}} \right) \\
 &= \frac{e^{-x}}{(1 - e^{-x})^2},
 \end{aligned}$$

for all $x > 0$. Thus, setting $x = 1$, we have

$$\sum_{n=0}^{\infty} n e^{-n} = \frac{e^{-1}}{(1 - e^{-1})^2}.$$